Continue work on AVL trees

examples/avl.v
@@ -1,57 +1,75 @@
 Require Import Arith ZArith Compare_dec.
 
 Section Tree.
-  Inductive tree (A: Type) : Type :=
-    | Leaf: tree A
-    | Node: A -> tree A -> tree A -> tree A.
+  Inductive tree (X: Type) : Type :=
+    | Leaf: tree X
+    | Node: X -> tree X -> tree X -> tree X.
 
-  Implicit Arguments Leaf [[A]].
-  Implicit Arguments Node [[A]].
+  Implicit Arguments Leaf [[X]].
+  Implicit Arguments Node [[X]].
 
-  Fixpoint node_count {A: Type} (t: tree A) : nat :=
+  Fixpoint node_count {X: Type} (t: tree X) : nat :=
     match t with
     | Leaf       => 0
-    | Node _ a b => 1 + node_count a + node_count b
+    | Node _ l r => 1 + node_count l + node_count r
     end.
 
-  Fixpoint tree_height {A: Type} (t: tree A) : nat :=
+  Fixpoint tree_height {X: Type} (t: tree X) : nat :=
     match t with
     | Leaf       => 0
-    | Node _ a b => 1 + max (tree_height a) (tree_height b)
+    | Node _ l r => 1 + max (tree_height l) (tree_height r)
   end.
 
-  Theorem tree_height_le_count: forall {A: Type}, forall t: tree A,
+  Theorem tree_height_le_count: forall {X: Type}, forall t: tree X,
     tree_height t <= node_count t.
   Proof.
-    intros X t. induction t as [| x a IHa b].
+    intros X t. induction t as [| x l IHl r IHr].
       simpl. reflexivity.
       simpl.
       apply Le.le_n_S.
       apply Max.max_case_strong.
-        intro H. rewrite IHa. apply le_plus_l.
-        intro H. rewrite IHb. apply le_plus_r.
+        intro H. rewrite IHl. apply le_plus_l.
+        intro H. rewrite IHr. apply le_plus_r.
   Qed.
 
   Section Search.
-    Inductive
+    Inductive In (x: nat) : tree nat -> Prop :=
+      | InRoot: forall y l r, eq_nat x y -> In x (Node y l r)
+      | InLeft: forall y l r, In x l -> In x (Node y l r)
+      | InRight: forall y l r, In x r -> In x (Node y l r).
+
+    Definition lt_tree x t := forall y: nat, In y t -> lt y x.
+    Definition gt_tree x t := forall y: nat, In y t -> gt y x.
+
+    Lemma lt_leaf: forall x, lt_tree x Leaf.
+    Proof. unfold lt_tree. intros. inversion H. Qed.
+
+    Lemma gt_leaf: forall x, gt_tree x Leaf.
+    Proof. unfold gt_tree. intros. inversion H. Qed.
+
+    Inductive BST: tree nat -> Prop :=
+      | bst_leaf: BST Leaf
+      | bst_node: forall x l r,
+        BST l -> BST r -> lt_tree x l -> gt_tree x r -> BST (Node x l r).
+    Hint Resolve bst_leaf bst_node: bst.
 
     Fixpoint search (x: nat) (t: tree nat) : option nat :=
       match t with
       | Leaf       => None
-      | Node y a b => match nat_compare x y with
-        | Lt => search x a
+      | Node y l r => match nat_compare x y with
+        | Lt => search x l
         | Eq => Some y
-        | Gt => search x b
+        | Gt => search x r
       end
     end.
 
     Fixpoint insert (x: nat) (t: tree nat) : tree nat :=
       match t with
       | Leaf       => Node x Leaf Leaf
-      | Node y a b => match nat_compare x y with
-        | Lt => Node y (insert x a) b
-        | Eq => Node x a b
-        | Gt => Node y a (insert x b)
+      | Node y l r => match nat_compare x y with
+        | Lt => Node y (insert x l) r
+        | Eq => Node x l r
+        | Gt => Node y l (insert x r)
       end
     end.
 
@@ -63,37 +81,48 @@ Section Tree.
         simpl. apply IHn'.
     Qed.
 
-    Theorem insert_search: forall (x: nat), forall (t: tree nat),
+    Theorem insert_search: forall (x: nat) (t: tree nat),
       search x (insert x t) = Some x.
     Proof.
-      intros x t. induction t as [| y a IHa b IHb].
+      intros x t. induction t as [| y l IHl r IHr].
         (* t = Leaf *)
         simpl. rewrite -> nat_compare_refl. reflexivity.
-        (* t = Node y a b *)
+        (* t = Node y l r *)
         simpl. remember (nat_compare x y) as eq. destruct eq.
           (* Eq *) simpl. rewrite nat_compare_refl. reflexivity.
-          (* Lt *) simpl. rewrite <- Heqeq. rewrite IHa. reflexivity.
-          (* Gt *) simpl. rewrite <- Heqeq. rewrite IHb. reflexivity.
+          (* Lt *) simpl. rewrite <- Heqeq. rewrite IHl. reflexivity.
+          (* Gt *) simpl. rewrite <- Heqeq. rewrite IHr. reflexivity.
     Qed.
+
+    Theorem insert_correct: forall (x: nat) (t: tree nat),
+      BST t -> BST (insert x t).
+    Proof.
+      intros x t H. induction t as [| y l IHl r IHr].
+        simpl.
+        apply bst_node.
+        auto with bst.
+        auto with bst.
+        auto with bst.
+        apply lt_leaf.
+        apply gt_leaf.
+        
   End Search.
 
   Section AVL.
     Open Scope Z_scope.
 
-    Definition balance_factor (t: tree A) : Z :=
+    Definition balance_factor {X: Type} (t: tree X) : Z :=
       match t with
       | Leaf       => 0
-      | Node a _ b => Z.of_nat (tree_height a) - Z.of_nat (tree_height b)
+      | Node _ l r => Z.of_nat (tree_height l) - Z.of_nat (tree_height r)
       end.
 
-    Definition is_balanced (t: tree A) : Prop :=
+    Definition is_balanced {X: Type} (t: tree X) : Prop :=
       -1 <= balance_factor t <= 1.
 
-    Inductive AVL : tree A -> Prop :=
+    Inductive AVL {X: Type} : tree X -> Prop :=
       | avl_nil: AVL Leaf
-      | avl_node: forall n, is_balanced n -> AVL n.
-
-    Fixpoint avl_insert (x: A) (t: tree A) : tree A :=
-      match
+      | avl_node: forall x l r,
+        AVL l -> AVL r -> is_balanced l -> is_balanced r -> AVL (Node x l r).
   End AVL.
 End Tree.
